Isabelle/Shelley/Cryptography.thy
@@ -4,6 +4,10 @@ theory Cryptography
   imports Main
 begin
 
+text \<open> Public verifying key \<close>
+
+typedecl v_key
+
 text \<open> Hash of a key \<close>
 
 typedecl key_hash
@@ -11,5 +15,9 @@ typedecl key_hash
 text \<open> Genesis key hash \<close>
 
 typedecl key_hash_g
+
+text \<open> hashKey function \<close>
+
+consts hash_key :: "v_key \<Rightarrow> key_hash"
 
 end
